theories/TM/Code/ListTM.v
@@ -1,4 +1,4 @@
-From Undecidability.TM.Code.List Require Export Nth Cons_constant App Length Rev.
+From Undecidability.TM.Code.List Require Export Nth Cons_constant App Length Rev Concat_Repeat.
 
 From Undecidability Require Import HoareLogic.
 Ltac hstep_ListTM :=
